Update Desargues_3D.thy

Space/Desargues_3D.thy
@@ -2,50 +2,69 @@ theory Desargues_3D
   imports Main Higher_Projective_Space_Rank_Axioms Matroid_Rank_Properties
 begin
 
+(*
+Contents:
+- We prove Desargues's theorem: if two triangles ABC and A'B'C' are perspective from a point P (ie. 
+the lines AA', BB' and CC' are concurrent in P), then they are perspective from a line (ie. the points
+\<alpha> = BC \<inter> B'C', \<beta> = AC \<inter> A'C' and \<gamma> = AB \<inter> A'B' are collinear).
+In this file we restrict ourself to the case where the two triangles ABC and A'B'C' are not coplanar. 
+*)
+
+definition desargues_config_3D :: "[Points, Points, Points, Points, Points, Points, Points, Points, Points, Points] => bool" 
+  where "desargues_config_3D A B C A' B' C' P \<alpha> \<beta> \<gamma> \<equiv> rk {A, B, C} = 3 \<and> rk {A', B', C'} = 3 \<and> 
+rk {A, A', P} = 2 \<and> rk {B, B', P} = 2 \<and> rk {C, C', P} = 2 \<and> rk {A, B, C, A', B', C'} \<ge> 4 \<and> 
+rk {B, C, \<alpha>} = 2 \<and> rk {B', C', \<alpha>} = 2 \<and> rk {A, C, \<beta>} = 2 \<and> rk {A', C', \<beta>} = 2 \<and> rk {A, B, \<gamma>} = 2 \<and>
+rk {A', B', \<gamma>} = 2"
+
 lemma coplanar_4 :
-  assumes "rk {A, B, C} = 3" and "rk {A', B', C'} = 3" and "rk {A, A', P} = 2" and "rk {B, B', P} = 2"
-    and "rk {C, C', P} = 2" and "rk {A, B, C, A', B', C'} \<ge> 4" and "rk {B, C, \<alpha>} = 2" 
-    and "rk {B', C', \<alpha>} = 2" and "rk {A, C, \<beta>} = 2" and "rk {A', C', \<beta>} = 2" and "rk {A, B, \<gamma>} = 2" 
-    and "rk {A', B', \<gamma>} = 2"
-  shows "rk {A, B, C, \<alpha>} = 3" and "rk {A', B', C', \<alpha>} = 3"
+  assumes "rk {A, B, C} = 3" and "rk {B, C, \<alpha>} = 2" 
+  shows "rk {A, B, C, \<alpha>} = 3"
 proof-
   have f1:"rk {A, B, C, \<alpha>} \<ge> 3" using matroid_ax_2
     by (metis assms(1) empty_subsetI insert_mono)
   have "rk {A, B, C, \<alpha>} + rk {B, C} \<le> rk {A, B, C} + rk {B, C, \<alpha>}" using matroid_ax_3_alt
-    by (metis Un_insert_right add_One_commute add_mono assms(1) assms(7) matroid_ax_2_alt nat_1_add_1 numeral_plus_one rk_singleton semiring_norm(3) sup_bot.right_neutral)
+    by (metis Un_insert_right add_One_commute add_mono assms(1) assms(2) matroid_ax_2_alt nat_1_add_1 numeral_plus_one rk_singleton semiring_norm(3) sup_bot.right_neutral)
   then have f2:"rk {A, B, C, \<alpha>} \<le> 3"
-    by (metis Un_insert_right add_One_commute assms(7) matroid_ax_2_alt numeral_plus_one semiring_norm(3) sup_bot.right_neutral)
+    by (metis Un_insert_right add_One_commute assms(2) matroid_ax_2_alt numeral_plus_one semiring_norm(3) sup_bot.right_neutral)
   from f1 and f2 show "rk {A, B, C, \<alpha>} = 3" by auto
-(* Note that the points A, B, C and A', B', C' have symmetric roles, so the same result holds for 
-the points A', B' and C' *)
-  thus "rk {A', B', C', \<alpha>} = 3"
-    by (smt One_nat_def Un_assoc Un_commute add.commute add_Suc_right antisym_conv assms(2) assms(8) insert_is_Un matroid_ax_2_alt nat_1_add_1 numeral_2_eq_2 numeral_3_eq_3)
+qed
+
+lemma desargues_config_3D_coplanar_4 :
+  assumes "desargues_config_3D A B C A' B' C' P \<alpha> \<beta> \<gamma>"
+  shows "rk {A, B, C, \<alpha>} = 3" and "rk {A', B', C', \<alpha>} = 3"
+proof-
+  show "rk {A, B, C, \<alpha>} = 3"
+    using assms desargues_config_3D_def[of A B C A' B' C' P \<alpha> \<beta> \<gamma>] coplanar_4 by blast
+  show "rk {A', B', C', \<alpha>} = 3"
+    using assms desargues_config_3D_def[of A B C A' B' C' P \<alpha> \<beta> \<gamma>] coplanar_4 by blast
 qed
 
 lemma coplanar_4_bis :
-  assumes "rk {A, B, C} = 3" and "rk {A', B', C'} = 3" and "rk {A, A', P} = 2" and "rk {B, B', P} = 2"
-    and "rk {C, C', P} = 2" and "rk {A, B, C, A', B', C'} \<ge> 4" and "rk {B, C, \<alpha>} = 2" 
-    and "rk {B', C', \<alpha>} = 2" and "rk {A, C, \<beta>} = 2" and "rk {A', C', \<beta>} = 2" and "rk {A, B, \<gamma>} = 2" 
-    and "rk {A', B', \<gamma>} = 2"
-  shows "rk {A, B, C, \<beta>} = 3" and "rk {A', B', C', \<beta>} = 3"
+  assumes "rk {A, B, C} = 3" and "rk {A, C, \<beta>} = 2"
+  shows "rk {A, B, C, \<beta>} = 3"
 proof-
   have f1:"rk {A, B, C, \<beta>} \<ge> 3" using matroid_ax_2
     by (metis assms(1) empty_subsetI insert_mono)
   have "rk {A, B, C, \<beta>} + rk {A, C} \<le> rk {A, B, C} + rk {A, C, \<beta>}" using matroid_ax_3_alt
-    by (smt One_nat_def add_Suc_right add_leD1 add_le_mono assms(1) assms(9) insert_commute insert_is_Un matroid_ax_3 numeral_2_eq_2 numeral_3_eq_3 one_add_one rk_singleton)
+    by (smt One_nat_def add_Suc_right add_leD1 add_le_mono assms(1) assms(2) insert_commute insert_is_Un matroid_ax_3 numeral_2_eq_2 numeral_3_eq_3 one_add_one rk_singleton)
   then have f2:"rk {A, B, C, \<beta>} \<le> 3"
-    by (smt One_nat_def Suc_le_mono add_le_cancel_right assms(1) assms(9) f1 insert_absorb2 insert_commute nat.inject numeral_2_eq_2 numeral_3_eq_3 rk_couple rk_singleton_bis)
+    by (smt One_nat_def Suc_le_mono add_le_cancel_right assms(1) assms(2) f1 insert_absorb2 insert_commute nat.inject numeral_2_eq_2 numeral_3_eq_3 rk_couple rk_singleton_bis)
   from f1 and f2 show "rk {A, B, C, \<beta>} = 3" by auto
-  thus "rk {A', B', C', \<beta>} = 3"
-    by (smt One_nat_def Un_assoc Un_commute add.commute add_Suc_right arith_special(3) assms(10) assms(2) insert_is_Un le_antisym matroid_ax_2_alt numeral_2_eq_2 numeral_3_eq_3)
+qed
+
+lemma desargues_config_3D_coplanar_4_bis :
+  assumes "desargues_config_3D A B C A' B' C' P \<alpha> \<beta> \<gamma>"
+  shows "rk {A, B, C, \<beta>} = 3" and "rk {A', B', C', \<beta>} = 3"
+proof-
+  show "rk {A, B, C, \<beta>} = 3"
+    using assms desargues_config_3D_def[of A B C A' B' C' P \<alpha> \<beta> \<gamma>] coplanar_4_bis by auto
+  show "rk {A', B', C', \<beta>} = 3"
+    using assms desargues_config_3D_def[of A B C A' B' C' P \<alpha> \<beta> \<gamma>] coplanar_4_bis by auto
 qed
 
 lemma coplanar_4_ter :
-  assumes "rk {A, B, C} = 3" and "rk {A', B', C'} = 3" and "rk {A, A', P} = 2" and "rk {B, B', P} = 2"
-    and "rk {C, C', P} = 2" and "rk {A, B, C, A', B', C'} \<ge> 4" and "rk {B, C, \<alpha>} = 2" 
-    and "rk {B', C', \<alpha>} = 2" and "rk {A, C, \<beta>} = 2" and "rk {A', C', \<beta>} = 2" and "rk {A, B, \<gamma>} = 2" 
-    and "rk {A', B', \<gamma>} = 2"
-  shows "rk {A, B, C, \<gamma>} = 3" and "rk {A', B', C', \<gamma>} = 3"
+  assumes "rk {A, B, C} = 3" and "rk {A, B, \<gamma>} = 2"
+  shows "rk {A, B, C, \<gamma>} = 3"
 proof-
   have f1:"rk {A, B, C, \<gamma>} \<ge> 3" using matroid_ax_2
     by (metis assms(1) empty_subsetI insert_mono)
@@ -53,107 +72,104 @@ proof-
     using matroid_ax_3_alt[of "{A, B}" "{A, B, C}" "{A, B, \<gamma>}"]
     by (simp add: insert_commute)
   then have f2:"rk {A, B, C, \<gamma>} \<le> 3"
-    by (smt One_nat_def Un_assoc Un_commute add.commute add_Suc_right assms(11) insert_is_Un matroid_ax_2_alt numeral_2_eq_2 numeral_3_eq_3 one_add_one)
+    by (smt One_nat_def Un_assoc Un_commute add.commute add_Suc_right assms(2) insert_is_Un matroid_ax_2_alt numeral_2_eq_2 numeral_3_eq_3 one_add_one)
   from f1 and f2 show "rk {A, B, C, \<gamma>} = 3" by auto
-  thus "rk {A', B', C', \<gamma>} = 3"
-    by (smt One_nat_def Un_assoc Un_commute add.commute add_Suc_right assms(12) assms(2) insert_is_Un le_antisym matroid_ax_2_alt nat_1_add_1 numeral_2_eq_2 numeral_3_eq_3)
+qed
+
+lemma desargues_config_3D_coplanar_4_ter :
+  assumes "desargues_config_3D A B C A' B' C' P \<alpha> \<beta> \<gamma>"
+  shows "rk {A, B, C, \<gamma>} = 3" and "rk {A', B', C', \<gamma>} = 3"
+proof-
+  show "rk {A, B, C, \<gamma>} = 3"
+    using assms desargues_config_3D_def[of A B C A' B' C' P \<alpha> \<beta> \<gamma>] coplanar_4_ter by auto
+  show "rk {A', B', C', \<gamma>} = 3"
+    using assms desargues_config_3D_def[of A B C A' B' C' P \<alpha> \<beta> \<gamma>] coplanar_4_ter by auto
 qed
 
 lemma coplanar_5 :
-  assumes "rk {A, B, C} = 3" and "rk {A', B', C'} = 3" and "rk {A, A', P} = 2" and "rk {B, B', P} = 2"
-    and "rk {C, C', P} = 2" and "rk {A, B, C, A', B', C'} \<ge> 4" and "rk {B, C, \<alpha>} = 2" 
-    and "rk {B', C', \<alpha>} = 2" and "rk {A, C, \<beta>} = 2" and "rk {A', C', \<beta>} = 2" and "rk {A, B, \<gamma>} = 2" 
-    and "rk {A', B', \<gamma>} = 2"
-  shows "rk {A, B, C, \<alpha>, \<beta>} = 3" and "rk {A', B', C', \<alpha>, \<beta>} = 3"
+  assumes "rk {A, B, C} = 3" and "rk {B, C, \<alpha>} = 2" and "rk {A, C, \<beta>} = 2"
+  shows "rk {A, B, C, \<alpha>, \<beta>} = 3"
 proof-
   have f1:"rk {A, B, C, \<alpha>} = 3" using coplanar_4
-    by (smt One_nat_def Un_assoc Un_commute add.commute add_Suc_right assms(1) assms(7) insert_is_Un le_antisym matroid_ax_2_alt numeral_2_eq_2 numeral_3_eq_3 one_add_one)
+    by (smt One_nat_def Un_assoc Un_commute add.commute add_Suc_right assms(1) assms(2) insert_is_Un le_antisym matroid_ax_2_alt numeral_2_eq_2 numeral_3_eq_3 one_add_one)
   have f2:"rk {A, B, C, \<beta>} = 3" using coplanar_4_bis
-    by (smt One_nat_def Un_assoc Un_commute add.commute add_Suc_right assms(1) assms(9) insert_is_Un le_antisym matroid_ax_2_alt numeral_2_eq_2 numeral_3_eq_3 one_add_one)
+    by (smt One_nat_def Un_assoc Un_commute add.commute add_Suc_right assms(1) assms(3) insert_is_Un le_antisym matroid_ax_2_alt numeral_2_eq_2 numeral_3_eq_3 one_add_one)
   from f1 and f2 show "rk {A, B, C, \<alpha>, \<beta>} = 3" 
     using matroid_ax_3_alt'
     by (metis Un_assoc assms(1) insert_is_Un)
-  have f1':"rk {A', B', C', \<alpha>} = 3" using coplanar_4
-    by (smt One_nat_def Un_assoc Un_commute add.commute add_Suc_right arith_special(3) assms(2) assms(8) insert_is_Un le_antisym matroid_ax_2_alt numeral_2_eq_2 numeral_3_eq_3)
-  have f2':"rk {A', B', C', \<beta>} = 3" using coplanar_4_bis
-    by (smt One_nat_def Un_commute add.commute add_Suc_right assms(10) assms(2) insert_commute insert_is_Un le_antisym matroid_ax_2_alt nat_1_add_1 numeral_2_eq_2 numeral_3_eq_3)
-  from f1' and f2' show "rk {A', B', C', \<alpha>, \<beta>} = 3"
-    using matroid_ax_3_alt'
-    by (metis Un_assoc assms(2) insert_is_Un)
 qed
 
+lemma desargues_config_3D_coplanar_5 :
+  assumes "desargues_config_3D A B C A' B' C' P \<alpha> \<beta> \<gamma>"
+  shows "rk {A, B, C, \<alpha>, \<beta>} = 3" and "rk {A', B', C', \<alpha>, \<beta>} = 3"
+proof-
+  show "rk {A, B, C, \<alpha>, \<beta>} = 3"
+    using assms desargues_config_3D_def coplanar_5 by auto
+  show "rk {A', B', C', \<alpha>, \<beta>} = 3"
+    using assms desargues_config_3D_def coplanar_5 by auto
+qed
+
+
 lemma coplanar_5_bis :
-  assumes "rk {A, B, C} = 3" and "rk {A', B', C'} = 3" and "rk {A, A', P} = 2" and "rk {B, B', P} = 2"
-    and "rk {C, C', P} = 2" and "rk {A, B, C, A', B', C'} \<ge> 4" and "rk {B, C, \<alpha>} = 2" 
-    and "rk {B', C', \<alpha>} = 2" and "rk {A, C, \<beta>} = 2" and "rk {A', C', \<beta>} = 2" and "rk {A, B, \<gamma>} = 2" 
-    and "rk {A', B', \<gamma>} = 2"
-  shows "rk {A, B, C, \<alpha>, \<gamma>} = 3" and "rk {A', B', C', \<alpha>, \<gamma>} = 3"
+  assumes "rk {A, B, C} = 3" and "rk {B, C, \<alpha>} = 2" and "rk {A, B, \<gamma>} = 2"
+  shows "rk {A, B, C, \<alpha>, \<gamma>} = 3"
 proof-
   have f1:"rk {A, B, C, \<alpha>} = 3" using coplanar_4
-    by (smt One_nat_def Un_assoc Un_commute add.commute add_Suc_right assms(1) assms(7) insert_is_Un le_antisym matroid_ax_2_alt numeral_2_eq_2 numeral_3_eq_3 one_add_one)
+    by (smt One_nat_def Un_assoc Un_commute add.commute add_Suc_right assms(1) assms(2) insert_is_Un le_antisym matroid_ax_2_alt numeral_2_eq_2 numeral_3_eq_3 one_add_one)
   have f2:"rk {A, B, C, \<gamma>} = 3" using coplanar_4_ter
-    by (smt One_nat_def Un_assoc Un_commute add.commute add_Suc_right assms(1) assms(11) insert_is_Un le_antisym matroid_ax_2_alt numeral_2_eq_2 numeral_3_eq_3 one_add_one)
+    by (smt One_nat_def Un_assoc Un_commute add.commute add_Suc_right assms(1) assms(3) insert_is_Un le_antisym matroid_ax_2_alt numeral_2_eq_2 numeral_3_eq_3 one_add_one)
   from f1 and f2 show "rk {A, B, C, \<alpha>, \<gamma>} = 3" 
     using matroid_ax_3_alt'
     by (metis Un_assoc assms(1) insert_is_Un)
-  have f1':"rk {A', B', C', \<alpha>} = 3" using coplanar_4
-    by (smt One_nat_def Un_assoc Un_commute add.commute add_Suc_right arith_special(3) assms(2) assms(8) insert_is_Un le_antisym matroid_ax_2_alt numeral_2_eq_2 numeral_3_eq_3)
-  have f2':"rk {A', B', C', \<gamma>} = 3" using coplanar_4_ter
-    by (smt One_nat_def Un_assoc Un_commute add.commute add_Suc_right arith_special(3) assms(12) assms(2) insert_is_Un le_antisym matroid_ax_2_alt numeral_2_eq_2 numeral_3_eq_3)
-  from f1' and f2' show "rk {A', B', C', \<alpha>, \<gamma>} = 3"
-    using matroid_ax_3_alt'
-    by (metis Un_assoc assms(2) insert_is_Un)
+qed
+
+lemma desargues_config_3D_coplanar_5_bis :
+  assumes "desargues_config_3D A B C A' B' C' P \<alpha> \<beta> \<gamma>"
+  shows "rk {A, B, C, \<alpha>, \<gamma>} = 3" and "rk {A', B', C', \<alpha>, \<gamma>} = 3"
+proof-
+  show "rk {A, B, C, \<alpha>, \<gamma>} = 3"
+    using assms desargues_config_3D_def[of A B C A' B' C' P \<alpha> \<beta> \<gamma>] coplanar_5_bis by auto
+  show "rk {A', B', C', \<alpha>, \<gamma>} = 3"
+    using assms desargues_config_3D_def[of A B C A' B' C' P \<alpha> \<beta> \<gamma>] coplanar_5_bis by auto
 qed
 
 lemma coplanar_6 :
-  assumes "rk {A, B, C} = 3" and "rk {A', B', C'} = 3" and "rk {A, A', P} = 2" and "rk {B, B', P} = 2"
-    and "rk {C, C', P} = 2" and "rk {A, B, C, A', B', C'} \<ge> 4" and "rk {B, C, \<alpha>} = 2" 
-    and "rk {B', C', \<alpha>} = 2" and "rk {A, C, \<beta>} = 2" and "rk {A', C', \<beta>} = 2" and "rk {A, B, \<gamma>} = 2" 
-    and "rk {A', B', \<gamma>} = 2"
-  shows "rk {A, B, C, \<alpha>, \<beta>, \<gamma>} = 3" and "rk {A', B', C', \<alpha>, \<beta>, \<gamma>} = 3"
+  assumes "rk {A, B, C} = 3" and "rk {B, C, \<alpha>} = 2" and "rk {A, B, \<gamma>} = 2" and "rk {A, C, \<beta>} = 2"
+  shows "rk {A, B, C, \<alpha>, \<beta>, \<gamma>} = 3"
 proof-
   have f1:"rk {A, B, C, \<alpha>, \<gamma>} = 3" 
-    using coplanar_5_bis[of A B C A' B' C' P \<alpha> \<beta> \<gamma>] assms(1) assms(10) assms(11) assms(12) assms(2) assms(3) assms(4) assms(5) assms(6) assms(7) assms(8) assms(9) 
-    by blast
+    using coplanar_5_bis assms(1) assms(2) assms(3) by auto
   have f2:"rk {A, B, C, \<alpha>, \<beta>} = 3"
-    using coplanar_5[of A B C A' B' C' P \<alpha> \<beta> \<gamma>] assms(1) assms(10) assms(11) assms(12) assms(2) assms(3) assms(4) assms(5) assms(6) assms(7) assms(8) assms(9) 
-    by blast
+    using coplanar_5 assms(1) assms(2) assms(4) by auto
   have f3:"rk {A, B, C, \<alpha>} = 3" 
-    using coplanar_4
-    by (smt One_nat_def Un_assoc Un_commute add.commute add_Suc_right assms(1) assms(7) insert_is_Un le_antisym matroid_ax_2_alt numeral_2_eq_2 numeral_3_eq_3 one_add_one)
+    using coplanar_4 assms(1) assms(2) by auto
   from f1 and f2 and f3 show "rk {A, B, C, \<alpha>, \<beta>, \<gamma>} = 3" 
     using matroid_ax_3_alt'[of "{A, B, C, \<alpha>}" "\<beta>" "\<gamma>"]
     by (metis Un_insert_left sup_bot.left_neutral)
-  have f1':"rk {A', B', C', \<alpha>, \<gamma>} = 3" 
-    using coplanar_5_bis[of A B C A' B' C' P \<alpha> \<beta> \<gamma>] assms(1) assms(10) assms(11) assms(12) assms(2) assms(3) assms(4) assms(5) assms(6) assms(7) assms(8) assms(9) 
-    by blast
-  have f2':"rk {A', B', C', \<alpha>, \<beta>} = 3"
-    using coplanar_5[of A B C A' B' C' P \<alpha> \<beta> \<gamma>] assms(1) assms(10) assms(11) assms(12) assms(2) assms(3) assms(4) assms(5) assms(6) assms(7) assms(8) assms(9) 
-    by blast
-  have f3':"rk {A', B', C', \<alpha>} = 3"
-    using coplanar_4
-    by (smt Un_commute Un_insert_left add_One_commute assms(2) assms(8) insert_is_Un le_antisym matroid_ax_2_alt numeral_plus_one semiring_norm(3))
-  from f1' f2' f3' show "rk {A', B', C', \<alpha>, \<beta>, \<gamma>} = 3"
-    using matroid_ax_3_alt'[of "{A', B', C', \<alpha>}" "\<beta>" "\<gamma>"]
-    by (metis Un_insert_left sup_bot.left_neutral)
 qed
 
-lemma non_coplanar :
-  assumes "rk {A, B, C} = 3" and "rk {A', B', C'} = 3" and "rk {A, A', P} = 2" and "rk {B, B', P} = 2"
-    and "rk {C, C', P} = 2" and "rk {A, B, C, A', B', C'} \<ge> 4" and "rk {B, C, \<alpha>} = 2" 
-    and "rk {B', C', \<alpha>} = 2" and "rk {A, C, \<beta>} = 2" and "rk {A', C', \<beta>} = 2" and "rk {A, B, \<gamma>} = 2" 
-    and "rk {A', B', \<gamma>} = 2"
+lemma desargues_config_3D_coplanar_6 :
+  assumes "desargues_config_3D A B C A' B' C' P \<alpha> \<beta> \<gamma>"
+  shows "rk {A, B, C, \<alpha>, \<beta>, \<gamma>} = 3" and "rk {A', B', C', \<alpha>, \<beta>, \<gamma>} = 3"
+proof-
+  show "rk {A, B, C, \<alpha>, \<beta>, \<gamma>} = 3"
+    using assms desargues_config_3D_def[of A B C A' B' C' P \<alpha> \<beta> \<gamma>] coplanar_6 by auto
+  show "rk {A', B', C', \<alpha>, \<beta>, \<gamma>} = 3"
+    using assms desargues_config_3D_def[of A B C A' B' C' P \<alpha> \<beta> \<gamma>] coplanar_6 by auto
+qed
+
+lemma desargues_config_3D_non_coplanar :
+  assumes "desargues_config_3D A B C A' B' C' P \<alpha> \<beta> \<gamma>"
   shows "rk {A, B, C, A', B', C', \<alpha>, \<beta>, \<gamma>} \<ge> 4" 
 proof-
-  have "rk {A, B, C, A', B', C'} \<le> rk {A, B, C, A', B', C', \<alpha>, \<beta>, \<gamma>}" using matroid_ax_2 by auto
-  thus "4 \<le> rk {A, B, C, A', B', C', \<alpha>, \<beta>, \<gamma>}" using matroid_ax_2 assms(6) by linarith
+  have "rk {A, B, C, A', B', C'} \<le> rk {A, B, C, A', B', C', \<alpha>, \<beta>, \<gamma>}" 
+    using matroid_ax_2 by auto
+  thus "4 \<le> rk {A, B, C, A', B', C', \<alpha>, \<beta>, \<gamma>}" 
+    using matroid_ax_2 assms desargues_config_3D_def[of A B C A' B' C' P \<alpha> \<beta> \<gamma>] by linarith
 qed
 
 theorem desargues_3D :
-  assumes "rk {A, B, C} = 3" and "rk {A', B', C'} = 3" and "rk {A, A', P} = 2" and "rk {B, B', P} = 2"
-    and "rk {C, C', P} = 2" and "rk {A, B, C, A', B', C'} \<ge> 4" and "rk {B, C, \<alpha>} = 2" 
-    and "rk {B', C', \<alpha>} = 2" and "rk {A, C, \<beta>} = 2" and "rk {A', C', \<beta>} = 2" and "rk {A, B, \<gamma>} = 2" 
-    and "rk {A', B', \<gamma>} = 2"
+  assumes "desargues_config_3D A B C A' B' C' P \<alpha> \<beta> \<gamma>"
   shows "rk {\<alpha>, \<beta>, \<gamma>} \<le> 2"
 proof-
   have "rk {A, B, C, A', B', C', \<alpha>, \<beta>, \<gamma>} + rk {\<alpha>, \<beta>, \<gamma>} \<le> rk {A, B, C, \<alpha>, \<beta>, \<gamma>} + rk {A', B', C', \<alpha>, \<beta>, \<gamma>}"
@@ -161,9 +177,11 @@ proof-
     by (simp add: insert_commute)
   then have "rk {\<alpha>, \<beta>, \<gamma>} \<le> rk {A, B, C, \<alpha>, \<beta>, \<gamma>} + rk {A', B', C', \<alpha>, \<beta>, \<gamma>} - rk {A, B, C, A', B', C', \<alpha>, \<beta>, \<gamma>}"
     by linarith
-  thus "rk {\<alpha>, \<beta>, \<gamma>} \<le> 2" using coplanar_6[of A B C A' B' C' P \<alpha> \<beta> \<gamma>] non_coplanar[of A B C A' B' C' P \<alpha> \<beta> \<gamma>]
-    by (smt Nat.le_add_diff \<open>rk {A, B, C, A', B', C', \<alpha>, \<beta>, \<gamma>} + rk {\<alpha>, \<beta>, \<gamma>} \<le> rk {A, B, C, \<alpha>, \<beta>, \<gamma>} + rk {A', B', C', \<alpha>, \<beta>, \<gamma>}\<close> add_diff_cancel_right' add_leD1 assms(1) assms(10) assms(11) assms(12) assms(2) assms(3) assms(4) assms(5) assms(6) assms(7) assms(8) assms(9) diff_diff_left le_add_diff_inverse numeral_plus_one semiring_norm(2) semiring_norm(5) semiring_norm(8))
+  thus "rk {\<alpha>, \<beta>, \<gamma>} \<le> 2" using assms desargues_config_3D_coplanar_6 desargues_config_3D_non_coplanar
+    by fastforce
 qed
+
+end
 
 
 
